---
title: 'Clebschâ€“Gordan coefficients'
date: 2024-04-29
permalink: /posts/2024/04/clebschgordan/
tags:
  - Clebsch-Gordan
---

Some useful results on Clebsch-Gordan coefficients ([see wiki for more](https://en.wikipedia.org/wiki/Clebsch%E2%80%93Gordan_coefficients)).

$$
\langle j_1m_1j_2m_2|00\rangle = \delta_{j_1j_2}\delta_{m_1,-m_2}\frac{(-1)^{j_1-m_1}}{\sqrt{[j_1]}},\quad
[j_1]\equiv 2j_1+1.
$$

$$
{\displaystyle {\begin{aligned}
\langle j_{1}\,m_{1}\,j_{2}\,m_{2}|J\,M\rangle &=(-1)^{j_{1}+j_{2}-J}\langle j_{1}\,(-m_{1})\,j_{2}\,(-m_{2})|J\,(-M)\rangle \\&=(-1)^{j_{1}+j_{2}-J}\langle j_{2}\,m_{2}\,j_{1}\,m_{1}|J\,M\rangle \\&=(-1)^{j_{1}-m_{1}}{\sqrt {\frac {2J+1}{2j_{2}+1}}}\langle j_{1}\,m_{1}\,J\,(-M)|j_{2}\,(-m_{2})\rangle \\&=(-1)^{j_{2}+m_{2}}{\sqrt {\frac {2J+1}{2j_{1}+1}}}\langle J\,(-M)\,j_{2}\,m_{2}|j_{1}\,(-m_{1})\rangle \\&=(-1)^{j_{1}-m_{1}}{\sqrt {\frac {2J+1}{2j_{2}+1}}}\langle J\,M\,j_{1}\,(-m_{1})|j_{2}\,m_{2}\rangle \\&=(-1)^{j_{2}+m_{2}}{\sqrt {\frac {2J+1}{2j_{1}+1}}}\langle j_{2}\,(-m_{2})\,J\,M|j_{1}\,m_{1}\rangle \end{aligned}}}
$$

$$
{\displaystyle \sum _{m}(-1)^{j-m}\langle j\,m\,j\,(-m)|J\,0\rangle =\delta _{J,0}{\sqrt {2j+1}}}
$$
